theories/Infra/Range.v
@@ -1,0 +1,80 @@
+Require Import CSet Util MoreList Take MoreInversion LengthEq.
+
+Fixpoint range (n d:nat) :=
+  match d with
+  | 0 => nil
+  | S d => n::range (S n) d
+  end.
+
+Lemma range_get k d n x
+  : get (range k d) n x
+    -> x = k + n.
+Proof.
+  intros. general induction d; simpl in *; isabsurd.
+  inv H. omega. eapply IHd in H4. omega.
+Qed.
+
+Lemma get_range k d n x
+  : x = k + n
+    -> n < d
+    -> get (range k d) n x.
+Proof.
+  intros. general induction d; simpl in *; isabsurd.
+  destruct n.
+  - orewrite (k + 0 = k). eauto using get.
+  - econstructor. eapply IHd; eauto. omega. omega.
+Qed.
+
+Ltac range_get_simpl :=
+  match goal with
+  | [H : get (range ?k ?d) ?n ?x |- _ ] =>
+    eapply range_get in H; try (is_var x; subst x)
+  end.
+
+Smpl Add range_get_simpl : inv_get.
+
+Lemma range_len k n
+  : ❬range k n❭ = n.
+Proof.
+  general induction n; simpl; eauto.
+Qed.
+
+Smpl Add rewrite range_len : len.
+
+Lemma x_notin_range x k n
+  : x ∉ of_list (range k n)
+    -> x < k \/ k+n <= x.
+Proof.
+  general induction n; simpl in *.
+  - decide (x < k); omega.
+  - decide (x = k); subst;
+      cset_tac'. eapply IHn in H1. destruct H1.
+    omega. omega.
+Qed.
+
+Lemma x_in_range x k n
+  : x >= k /\ k+n > x -> x ∈ of_list (range k n).
+Proof.
+  general induction n; simpl in *; dcr.
+  - exfalso; omega.
+  - decide (x = k); subst;
+      cset_tac'. eapply IHn. omega.
+Qed.
+
+Lemma in_range_x x k n
+  : x ∈ of_list (range k n) -> x >= k /\ k+n > x.
+Proof.
+  general induction n; simpl in *; dcr.
+  - cset_tac.
+  - decide (x = k); subst; try omega.
+    cset_tac'; eapply IHn in H0; omega.
+Qed.
+
+
+Lemma take_range k n d
+  : Take.take k (range n d) = range n (min k d).
+Proof.
+  general induction k; simpl; eauto.
+  repeat cases; eauto.
+  simpl in *. f_equal; eauto.
+Qed.
