theories/Reachability/ReachabilityAnalysisCorrect.v
@@ -4,7 +4,7 @@ Require Import Plus Util AllInRel Map CSet OptionR MoreList.
 Require Import Val Var Env IL Annotation AnnotationLattice Infra.Lattice.
 Require Import DecSolve Analysis Filter Terminating ContextMap.
 Require Import Analysis AnalysisForward FiniteFixpointIteration.
-Require Import Reachability ReachabilityAnalysis Subterm.
+Require Import Reachability ReachabilityAnalysis Subterm Range.
 
 Set Implicit Arguments.
 
